\documentclass[a4j, 12pt]{jarticle}
\usepackage{amsmath}
\usepackage{amssymb}
\usepackage{amsthm}

\begin{document}
$ ( \tan \theta)' = \frac{1}{\cos^2 \theta} $ より、

\begin{eqnarray}
 ( \tan \theta ・ \frac{1}{\cos^{n-2} \theta}) 
& = & \frac{1}{\cos^n \theta} +  \tan \theta ・  \frac{2-n}{\cos^{n-1} \theta} ・ ( - \sin \theta) \\
& = & \frac{1}{\cos^n \theta} +  \frac{n-2}{\cos^{n} \theta} ・ \sin^2 \theta \\
& = & \frac{1}{\cos^n \theta} +  \frac{n-2}{\cos^{n} \theta} ・ (1 -  \cos^2 \theta ) \\
& = & \frac{1}{\cos^n \theta} +  \frac{n-2}{\cos^{n} \theta} + \frac{n-2}{\cos^{n-2} \theta} \\
& = & \frac{n-1}{\cos^{n} \theta} + \frac{n-2}{\cos^{n-2} \theta} \\
\end{eqnarray}

この式の両辺を０から$\frac{\pi}{3}$ まで積分する。

\begin{eqnarray}
(右辺）　
& = & \int_{0}^{\frac{\pi}{3}} \frac{n-1}{\cos^{n} \theta} + \frac{n-2}{\cos^{n-2} \theta} \\
& = & 
\end{eqnarray}


\end{document}